src/StVM.v
@@ -12,10 +12,10 @@ Import ListNotations.
 (* Specific VM monad state *)
 (*Definition ev_store := MapC nat EvidenceC. *)
 Record cvm_st : Type := mk_st
-                          {st_ev:EvidenceC ;
+                          {st_ev:EvC ;
                            (*st_evT: Evidence ; *)
                            st_trace:list Ev ;
                            st_pl:Plc (*;
                            st_store:ev_store*)}.
 
-Definition empty_vmst := mk_st mtc [] 0 (* [] *) .
+Definition empty_vmst := mk_st (evc [] mt) [] 0 (* [] *) .
